more work on typing
define variables used by expressions and show that typing is precise
provided all used variables are initialised. Moreover show that the set
of initialised variables is monoton during program execution.

bil_envScript.sml
@@ -87,20 +87,6 @@ COND_CASES_TAC >> REWRITE_TAC[] >>
 Cases_on `env` >> SIMP_TAC std_ss [bil_env_update_def])
 
 
-val bil_env_var_is_bound_def = Define `
-  (bil_env_var_is_bound var IrregularEnv = F) /\
-  (bil_env_var_is_bound var (RegularEnv env) = (var IN FDOM env))`
-
-
-val bin_env_var_is_bound_ALT_DEF = store_thm ("bin_env_var_is_bound_ALT_DEF",
-  ``!var env. bil_env_var_is_bound var env <=> IS_SOME (bil_env_lookup_type var env)``,
-
-Cases_on `env` >> (
-  SIMP_TAC (std_ss++boolSimps.LIFT_COND_ss) [bil_env_var_is_bound_def, bil_env_var_is_bound_def,
-    bil_env_lookup_type_def, bil_env_lookup_def, FLOOKUP_DEF]
-));
-
-
 val is_valid_env_lookup = store_thm ("is_valid_env_lookup",
   ``!env vn ty v. is_valid_env env ==>
                   (bil_env_lookup vn env = SOME (ty, SOME v)) ==>
@@ -137,5 +123,198 @@ rename1 `r = Unknown` >>
 `type_of_bil_val r = SOME (bil_var_type v)` by METIS_TAC[is_valid_env_lookup] >>
 STRIP_TAC >>
 FULL_SIMP_TAC std_ss [type_of_bil_val_def]);
+
+
+
+
+val bil_env_varname_is_bound_def = Define `
+  (bil_env_varname_is_bound IrregularEnv var = F) /\
+  (bil_env_varname_is_bound (RegularEnv env) var = (var IN FDOM env))`;
+
+val bil_env_varname_is_bound_ALT_DEF = store_thm ("bil_env_varname_is_bound_ALT_DEF",
+  ``!var env. bil_env_varname_is_bound env var <=> IS_SOME (bil_env_lookup_type var env)``,
+
+Cases_on `env` >> (
+  SIMP_TAC (std_ss++boolSimps.LIFT_COND_ss) [bil_env_varname_is_bound_def,
+    bil_env_lookup_type_def, bil_env_lookup_def, FLOOKUP_DEF]
+));
+
+val bil_env_varname_is_bound_ALT2_DEF = store_thm ("bil_env_varname_is_bound_ALT2_DEF",
+  ``!var env. bil_env_varname_is_bound env var <=> IS_SOME (bil_env_lookup var env)``,
+
+SIMP_TAC std_ss [bil_env_varname_is_bound_ALT_DEF, bil_env_lookup_type_def,
+  optionTheory.IS_SOME_MAP]);
+
+
+val bil_env_var_is_declared_def = Define `
+  (bil_env_var_is_declared env (Var vn ty) <=>
+  (bil_env_lookup_type vn env = SOME ty))`;
+
+val bil_env_var_is_initialised_def = Define `
+  (bil_env_var_is_initialised env (Var vn ty) <=>
+  (?v. bil_env_lookup vn env = SOME (ty, SOME v)))`;
+
+
+val bil_env_var_is_initialised_weaken = store_thm ("bil_env_var_is_initialised_weaken",
+  ``!v env. bil_env_var_is_initialised env v ==> bil_env_var_is_declared env v``,
+Cases >> SIMP_TAC std_ss [bil_env_var_is_initialised_def, bil_env_var_is_declared_def,
+  GSYM LEFT_FORALL_IMP_THM, bil_env_lookup_type_def]);
+
+
+val bil_env_var_is_declared_weaken = store_thm ("bil_env_var_is_declared_weaken",
+  ``!v env. bil_env_var_is_declared env v ==> bil_env_varname_is_bound env (bil_var_name v)``,
+Cases >> SIMP_TAC std_ss [bil_env_var_is_declared_def,
+  GSYM LEFT_FORALL_IMP_THM, bil_env_varname_is_bound_ALT_DEF,
+  bil_var_name_def]);
+
+
+val _ = Datatype `bil_env_cond_t =
+  | EnvCond_varname_bound string
+  | EnvCond_var_declared bil_var_t
+  | EnvCond_var_initialised bil_var_t`;
+
+val bil_env_cond_eval_def = Define `
+  (bil_env_cond_eval env (EnvCond_varname_bound vn)  <=> bil_env_varname_is_bound   env vn) /\
+  (bil_env_cond_eval env (EnvCond_var_initialised v) <=> bil_env_var_is_initialised env v) /\
+  (bil_env_cond_eval env (EnvCond_var_declared v)    <=> bil_env_var_is_declared    env v)`;
+
+
+val bil_env_order_def = Define `
+  ((bil_env_order env1 env2) <=>
+     !vn ty vo. (bil_env_lookup vn env1 = SOME (ty, vo)) ==>
+                (?vo'. (bil_env_lookup vn env2 = SOME (ty, vo')) /\
+                       (IS_SOME vo ==> IS_SOME vo')))`;
+
+val bil_env_order_REFL = store_thm ("bil_env_order_REFL",
+  ``!env. bil_env_order env env``,
+SIMP_TAC std_ss [bil_env_order_def]);
+
+val bil_env_order_TRANS = store_thm ("bil_env_order_TRANS",
+  ``!env1 env2 env3.
+       bil_env_order env1 env2 ==> bil_env_order env2 env3 ==>
+       bil_env_order env1 env3``,
+SIMP_TAC std_ss [bil_env_order_def] >>
+METIS_TAC[]);
+
+
+val bil_env_varname_is_bound_ORDER = store_thm ("bil_env_varname_is_bound_ORDER",
+  ``!env1 env2 v. bil_env_order env1 env2 ==>
+                  bil_env_varname_is_bound env1 v ==>
+                  bil_env_varname_is_bound env2 v``,
+SIMP_TAC (std_ss++QI_ss) [bil_env_varname_is_bound_ALT_DEF, bil_env_order_def,
+  bil_env_lookup_type_def, optionTheory.IS_SOME_EXISTS] >>
+METIS_TAC[]);
+
+
+val bil_env_var_is_declared_ORDER = store_thm ("bil_env_var_is_declared_ORDER",
+  ``!env1 env2 v. bil_env_order env1 env2 ==>
+                  bil_env_var_is_declared env1 v ==>
+                  bil_env_var_is_declared env2 v``,
+Cases_on `v` >>
+SIMP_TAC (std_ss++QI_ss) [bil_env_var_is_declared_def, bil_env_order_def,
+  bil_env_lookup_type_def] >>
+METIS_TAC[]);
+
+
+val bil_env_var_is_initialised_ORDER = store_thm ("bil_env_var_is_initialised_ORDER",
+  ``!env1 env2 v. bil_env_order env1 env2 ==>
+                  bil_env_var_is_initialised env1 v ==>
+                  bil_env_var_is_initialised env2 v``,
+Cases_on `v` >>
+SIMP_TAC (std_ss) [bil_env_var_is_initialised_def, bil_env_order_def,
+  optionTheory.IS_SOME_EXISTS] >>
+METIS_TAC[]);
+
+
+val bil_env_cond_eval_ORDER = store_thm ("bil_env_cond_eval_ORDER",
+  ``!env1 env2 c. bil_env_order env1 env2 ==>
+                  bil_env_cond_eval env1 c ==>
+                  bil_env_cond_eval env2 c``,
+
+Cases_on `c` >> (
+  SIMP_TAC std_ss [bil_env_cond_eval_def] >>
+  METIS_TAC[bil_env_varname_is_bound_ORDER,
+            bil_env_var_is_declared_ORDER,
+            bil_env_var_is_initialised_ORDER]
+));
+
+
+val bil_env_vars_are_initialised_def = Define `
+  bil_env_vars_are_initialised env vs <=>
+  (!v. v IN vs ==> bil_env_var_is_initialised env v)`;
+
+val bil_env_vars_are_initialised_EMPTY = store_thm ("bil_env_vars_are_initialised_EMPTY",
+  ``!env. bil_env_vars_are_initialised env {}``,
+SIMP_TAC std_ss [bil_env_vars_are_initialised_def, pred_setTheory.NOT_IN_EMPTY]);
+
+val bil_env_vars_are_initialised_INSERT = store_thm ("bil_env_vars_are_initialised_INSERT",
+  ``!env v vs. bil_env_vars_are_initialised env (v INSERT vs) <=>
+               (bil_env_var_is_initialised env v /\ bil_env_vars_are_initialised env vs)``,
+SIMP_TAC std_ss [bil_env_vars_are_initialised_def, pred_setTheory.IN_INSERT] >>
+METIS_TAC[]);
+
+val bil_env_vars_are_initialised_UNION = store_thm ("bil_env_vars_are_initialised_UNION",
+  ``!env vs1 vs2. bil_env_vars_are_initialised env (vs1 UNION vs2) <=>
+                  (bil_env_vars_are_initialised env vs1 /\
+                   bil_env_vars_are_initialised env vs2) ``,
+SIMP_TAC std_ss [bil_env_vars_are_initialised_def, pred_setTheory.IN_UNION] >>
+METIS_TAC[]);
+
+val bil_env_vars_are_initialised_SUBSET = store_thm ("bil_env_vars_are_initialised_SUBSET",
+  ``!env vs1 vs2. bil_env_vars_are_initialised env vs1 ==>
+                  (vs2 SUBSET vs1) ==>
+                   bil_env_vars_are_initialised env vs2``,
+SIMP_TAC std_ss [bil_env_vars_are_initialised_def, pred_setTheory.SUBSET_DEF] >>
+METIS_TAC[]);
+
+
+val bil_env_vars_are_initialised_ORDER = store_thm ("bil_env_vars_are_initialised_ORDER",
+  ``!env1 env2 vs. bil_env_order env1 env2 ==>
+                   bil_env_vars_are_initialised env1 vs ==>
+                   bil_env_vars_are_initialised env2 vs``,
+
+SIMP_TAC std_ss [bil_env_vars_are_initialised_def] >>
+METIS_TAC[bil_env_var_is_initialised_ORDER]);
+
+
+val bil_env_order_update = store_thm ("bil_env_order_update",
+``!env vn vo ty.
+    ~(bil_env_varname_is_bound env vn) /\
+    (!v. (vo = SOME v) ==> (type_of_bil_val v = SOME ty)) ==>
+    bil_env_order env (bil_env_update vn vo ty env)``,
+
+Cases_on `env` >> (
+  SIMP_TAC std_ss [bil_env_update_def, bil_env_order_REFL,
+    bil_env_varname_is_bound_ALT_DEF]
+) >>
+REPEAT STRIP_TAC >>
+Cases_on `vo` >> (
+  FULL_SIMP_TAC (std_ss++boolSimps.LIFT_COND_ss) [
+    bil_env_lookup_type_def,
+    bil_env_lookup_def, bil_env_order_def,
+    finite_mapTheory.FLOOKUP_UPDATE]
+));
+
+
+val bil_env_order_write = store_thm ("bil_env_order_write",
+``!env v va.
+    is_env_regular (bil_env_write v va env) ==>
+    bil_env_order env (bil_env_write v va env)``,
+
+SIMP_TAC std_ss [bil_env_write_def] >>
+REPEAT STRIP_TAC >>
+COND_CASES_TAC >> FULL_SIMP_TAC std_ss [is_env_regular_def] >>
+Cases_on `env` >> (
+  FULL_SIMP_TAC std_ss [bil_env_update_def, bil_env_order_REFL]
+) >>
+FULL_SIMP_TAC std_ss [bil_env_check_type_def, bil_env_lookup_type_def] >>
+rename1 `SOME (FST xx)` >> Cases_on `xx` >> rename1 `FST (ty, vo)` >>
+Cases_on `SOME ty = type_of_bil_val va` >> FULL_SIMP_TAC std_ss [is_env_regular_def] >>
+FULL_SIMP_TAC (std_ss++boolSimps.LIFT_COND_ss) [
+    bil_env_order_def, bil_env_lookup_def,
+    finite_mapTheory.FLOOKUP_UPDATE]
+);
+
+
 
 val _ = export_theory();
