bil_typingScript.sml
@@ -123,6 +123,9 @@ val type_of_bil_exp_EQ_SOME_REWRS = store_thm ("type_of_bil_exp_EQ_SOME_REWRS",`
 
   (!v ty. (type_of_bil_exp (Den v) = SOME ty) <=> (ty = bil_var_type v)) /\
 
+  (!ct e ty ty'. (type_of_bil_exp (Cast ct e ty') = SOME ty) <=> (
+     (ty = ImmType ty') /\ (?it. (type_of_bil_exp e = SOME (ImmType it))))) /\
+
   (!et e ty. (type_of_bil_exp (UnaryExp et e) = SOME ty) <=> (
      (bil_type_is_ImmType ty) /\ (type_of_bil_exp e = SOME ty))) /\
 
@@ -132,6 +135,11 @@ val type_of_bil_exp_EQ_SOME_REWRS = store_thm ("type_of_bil_exp_EQ_SOME_REWRS",`
   (!pt e1 e2 ty. (type_of_bil_exp (BinPred pt e1 e2) = SOME ty) <=> (
      (ty = BoolType) /\ (?it. (type_of_bil_exp e1 = SOME (ImmType it)) /\
                               (type_of_bil_exp e2 = SOME (ImmType it))))) /\
+
+  (!ce e1 e2 ty. (type_of_bil_exp (IfThenElse ce e1 e2) = SOME ty) <=> (
+     (type_of_bil_exp ce = SOME BoolType) /\
+     (type_of_bil_exp e1 = SOME ty) /\
+     (type_of_bil_exp e2 = SOME ty))) /\
 
   (!rty ty ae en me. (type_of_bil_exp (Load me ae en rty) = SOME ty) <=> (
      (ty = ImmType rty) /\ (?at vt. (type_of_bil_exp me = SOME (MemType at vt)) /\
@@ -151,10 +159,17 @@ val type_of_bil_exp_EQ_SOME_REWRS = store_thm ("type_of_bil_exp_EQ_SOME_REWRS",`
 REPEAT CONJ_TAC >> (
   SIMP_TAC (std_ss++boolSimps.EQUIV_EXTRACT_ss) [type_of_bil_exp_def]
 ) >- (
+  REPEAT GEN_TAC >> REPEAT CASE_TAC >>
+    FULL_SIMP_TAC (std_ss++bil_type_ss) [bil_type_is_ImmType_def] >> METIS_TAC[]
+) >- (
   REPEAT GEN_TAC >> REPEAT CASE_TAC >> METIS_TAC[]
 ) >- (
   REPEAT GEN_TAC >> REPEAT CASE_TAC >> (
     FULL_SIMP_TAC std_ss [] >> METIS_TAC[]
+  )
+) >- (
+  REPEAT GEN_TAC >> REPEAT CASE_TAC >> (
+    FULL_SIMP_TAC std_ss [bil_type_is_ImmType_def] >> METIS_TAC[]
   )
 ) >- (
   REPEAT GEN_TAC >> REPEAT CASE_TAC >> (
@@ -169,10 +184,13 @@ REPEAT CONJ_TAC >> (
 
 
 
-val type_of_bil_exp_EQ_NONE_REWRS = store_thm ("type_of_bil_exp_EQ_NONE",``
+val type_of_bil_exp_EQ_NONE_REWRS = store_thm ("type_of_bil_exp_EQ_NONE_REWRS",``
   (!i. ~(type_of_bil_exp (Const i) = NONE)) /\
 
   (!v. ~(type_of_bil_exp (Den v) = NONE)) /\
+
+  (!ct e ty ty'. (type_of_bil_exp (Cast ct e ty') = NONE) <=> (
+     (!ity. (type_of_bil_exp e <> SOME (ImmType ity))))) /\
 
   (!et e. (type_of_bil_exp (UnaryExp et e) = NONE) <=> (
      (!ity. type_of_bil_exp e <> SOME (ImmType ity)))) /\
@@ -184,6 +202,11 @@ val type_of_bil_exp_EQ_NONE_REWRS = store_thm ("type_of_bil_exp_EQ_NONE",``
   (!pt e1 e2. (type_of_bil_exp (BinPred pt e1 e2) = NONE) <=> !ity.
      (type_of_bil_exp e1 <> SOME (ImmType ity)) \/
      (type_of_bil_exp e2 <> SOME (ImmType ity))) /\
+
+  (!ce e1 e2 ty. (type_of_bil_exp (IfThenElse ce e1 e2) = NONE) <=> (
+     (type_of_bil_exp ce <> SOME BoolType) \/
+     (type_of_bil_exp e1 = NONE) \/
+     (type_of_bil_exp e2 <> type_of_bil_exp e1))) /\
 
   (!rty ty ae en me. (type_of_bil_exp (Load me ae en rty) = NONE) <=> (
      (!at vt. (type_of_bil_exp me = SOME (MemType at vt)) /\
@@ -205,6 +228,8 @@ REPEAT CONJ_TAC >> (
 ) >- (
   REPEAT GEN_TAC >> REPEAT CASE_TAC >> FULL_SIMP_TAC (std_ss++bil_type_ss) [bil_type_is_ImmType_def]
 ) >- (
+  REPEAT GEN_TAC >> REPEAT CASE_TAC >> FULL_SIMP_TAC (std_ss++bil_type_ss) [bil_type_is_ImmType_def]
+) >- (
   REPEAT GEN_TAC >> REPEAT CASE_TAC >> (
     FULL_SIMP_TAC (std_ss++bil_type_ss) [bil_type_is_ImmType_def] >>
     METIS_TAC[]
@@ -213,6 +238,10 @@ REPEAT CONJ_TAC >> (
   REPEAT GEN_TAC >> REPEAT CASE_TAC >> (
     FULL_SIMP_TAC (std_ss++bil_type_ss) [bil_type_is_ImmType_def] >>
     METIS_TAC[]
+  )
+) >- (
+  REPEAT GEN_TAC >> REPEAT CASE_TAC >> (
+    FULL_SIMP_TAC (std_ss) []
   )
 ) >- (
   REPEAT GEN_TAC >> REPEAT CASE_TAC >> METIS_TAC[]
@@ -223,6 +252,79 @@ REPEAT CONJ_TAC >> (
 
 
 val bil_is_well_typed_exp_def = Define `bil_is_well_typed_exp e <=>  (type_of_bil_exp e <> NONE)`
+
+
+(* ------------------------------------------------------------------------- *)
+(*  Looking at  variables used somewhere in an expression                    *)
+(* ------------------------------------------------------------------------- *)
+
+val bil_vars_of_exp_def = Define `
+  (bil_vars_of_exp (Const _) = {}) /\
+  (bil_vars_of_exp (Den v) = {v}) /\
+  (bil_vars_of_exp (Cast _ e _) = bil_vars_of_exp e) /\
+  (bil_vars_of_exp (UnaryExp _ e) = bil_vars_of_exp e) /\
+  (bil_vars_of_exp (BinExp _ e1 e2) = (bil_vars_of_exp e1 UNION bil_vars_of_exp e2)) /\
+  (bil_vars_of_exp (BinPred _ e1 e2) = (bil_vars_of_exp e1 UNION bil_vars_of_exp e2)) /\
+  (bil_vars_of_exp (IfThenElse ec e1 e2) = (bil_vars_of_exp ec UNION bil_vars_of_exp e1 UNION bil_vars_of_exp e2)) /\
+  (bil_vars_of_exp (Load me ae _ _) = (bil_vars_of_exp me UNION bil_vars_of_exp ae)) /\
+  (bil_vars_of_exp (Store me ae _ ve) = (bil_vars_of_exp me UNION bil_vars_of_exp ae UNION bil_vars_of_exp ve))`
+
+
+val type_of_bil_exp_THM_with_init_vars = store_thm ("type_of_bil_exp_THM_with_init_vars",
+  ``!env. (is_valid_env env) ==>
+          (!e ty. (type_of_bil_exp e = SOME ty) ==>
+                  (bil_env_vars_are_initialised env (bil_vars_of_exp e)) ==>
+                  (type_of_bil_val (bil_eval_exp e env) = SOME ty))``,
+
+GEN_TAC >> STRIP_TAC >> Induct >> (
+  SIMP_TAC (std_ss++bil_val_ss) [bil_eval_exp_def, BoolType_def,
+    type_of_bil_exp_EQ_SOME_REWRS, bil_vars_of_exp_def,
+    bil_env_vars_are_initialised_UNION, bil_env_vars_are_initialised_INSERT,
+    bil_env_vars_are_initialised_EMPTY, PULL_EXISTS, PULL_FORALL, bil_type_is_ImmType_def] >>
+  REPEAT STRIP_TAC >>
+  FULL_SIMP_TAC (std_ss++bil_val_ss) [type_of_bil_val_EQ_ELIMS, bil_type_is_ImmType_def]
+) >- (
+  rename1 `bil_env_read v env` >>
+  Cases_on `v` >>
+  FULL_SIMP_TAC std_ss [bil_env_read_def, bil_env_var_is_initialised_def, bil_var_name_def,
+    bil_var_type_def, pairTheory.pair_case_thm] >>
+  METIS_TAC[is_valid_env_lookup]
+) >- (
+  SIMP_TAC (std_ss++bil_val_ss) [bil_eval_cast_REWRS, type_of_bil_gencast]
+) >- (
+  ASM_SIMP_TAC (std_ss++bil_val_ss) [bil_eval_unary_exp_REWRS, type_of_bil_unary_exp]
+) >- (
+  ASM_SIMP_TAC (std_ss++bil_val_ss) [bil_eval_bin_exp_REWRS, type_of_bil_bin_exp]
+) >- (
+  ASM_SIMP_TAC (std_ss++bil_val_ss) [bil_eval_bin_pred_REWRS, type_of_bil_val_def,
+    type_of_bool2b, BoolType_def]
+) >- (
+  ASM_SIMP_TAC (std_ss++bil_val_ss) [bil_eval_ifthenelse_REWRS] >>
+  METIS_TAC[]
+) >- (
+  ASM_SIMP_TAC (std_ss++bil_val_ss) [bil_eval_load_BASIC_REWR] >>
+  rename1 `bil_load_from_mem vt ity mmap en (b2n i)` >>
+  Cases_on `bil_load_from_mem vt ity mmap en (b2n i)` >- (
+    POP_ASSUM MP_TAC >>
+    ASM_SIMP_TAC (std_ss++bil_val_ss) [bil_load_from_mem_EQ_NONE] >>
+    Cases_on `en = NoEndian` >> (
+       FULL_SIMP_TAC (std_ss++boolSimps.CONJ_ss) [bil_number_of_mem_splits_ID]
+    )
+  ) >>
+  ASM_SIMP_TAC (std_ss++bil_val_ss) [] >>
+  METIS_TAC [type_of_bil_load_from_mem]
+) >- (
+  ASM_SIMP_TAC (std_ss++bil_val_ss) [bil_eval_store_BASIC_REWR] >>
+  rename1 `bil_store_in_mem vt ity mmap en (b2n i)` >>
+  Cases_on `bil_store_in_mem vt ity mmap en (b2n i)` >- (
+    POP_ASSUM MP_TAC >>
+    ASM_SIMP_TAC (std_ss++bil_val_ss) [bil_store_in_mem_EQ_NONE] >>
+    Cases_on `en = NoEndian` >> (
+       FULL_SIMP_TAC (std_ss++boolSimps.CONJ_ss) [bil_number_of_mem_splits_ID]
+    )
+  ) >>
+  ASM_SIMP_TAC (std_ss++bil_val_ss) []
+));
 
 
 
@@ -263,6 +365,64 @@ REPEAT STRIP_TAC >>
 `MEM bl p` by METIS_TAC [bil_get_program_block_info_by_label_THM, listTheory.MEM_EL] >>
 FULL_SIMP_TAC std_ss [listTheory.EVERY_MEM] >>
 METIS_TAC[]);
+
+
+val type_of_bil_exp_THM_with_init_vars = store_thm ("type_of_bil_exp_THM_with_init_vars",
+  ``!env. (is_valid_env env) ==>
+          (!e ty. (type_of_bil_exp e = SOME ty) ==>
+                  (bil_env_vars_are_initialised env (bil_vars_of_exp e)) ==>
+                  (type_of_bil_val (bil_eval_exp e env) = SOME ty))``,
+
+GEN_TAC >> STRIP_TAC >> Induct >> (
+  SIMP_TAC (std_ss++bil_val_ss) [bil_eval_exp_def, BoolType_def,
+    type_of_bil_exp_EQ_SOME_REWRS, bil_vars_of_exp_def,
+    bil_env_vars_are_initialised_UNION, bil_env_vars_are_initialised_INSERT,
+    bil_env_vars_are_initialised_EMPTY, PULL_EXISTS, PULL_FORALL, bil_type_is_ImmType_def] >>
+  REPEAT STRIP_TAC >>
+  FULL_SIMP_TAC (std_ss++bil_val_ss) [type_of_bil_val_EQ_ELIMS, bil_type_is_ImmType_def]
+) >- (
+  rename1 `bil_env_read v env` >>
+  Cases_on `v` >>
+  FULL_SIMP_TAC std_ss [bil_env_read_def, bil_env_var_is_initialised_def, bil_var_name_def,
+    bil_var_type_def, pairTheory.pair_case_thm] >>
+  METIS_TAC[is_valid_env_lookup]
+) >- (
+  SIMP_TAC (std_ss++bil_val_ss) [bil_eval_cast_REWRS, type_of_bil_gencast]
+) >- (
+  ASM_SIMP_TAC (std_ss++bil_val_ss) [bil_eval_unary_exp_REWRS, type_of_bil_unary_exp]
+) >- (
+  ASM_SIMP_TAC (std_ss++bil_val_ss) [bil_eval_bin_exp_REWRS, type_of_bil_bin_exp]
+) >- (
+  ASM_SIMP_TAC (std_ss++bil_val_ss) [bil_eval_bin_pred_REWRS, type_of_bil_val_def,
+    type_of_bool2b, BoolType_def]
+) >- (
+  ASM_SIMP_TAC (std_ss++bil_val_ss) [bil_eval_ifthenelse_REWRS] >>
+  METIS_TAC[]
+) >- (
+  ASM_SIMP_TAC (std_ss++bil_val_ss) [bil_eval_load_BASIC_REWR] >>
+  rename1 `bil_load_from_mem vt ity mmap en (b2n i)` >>
+  Cases_on `bil_load_from_mem vt ity mmap en (b2n i)` >- (
+    POP_ASSUM MP_TAC >>
+    ASM_SIMP_TAC (std_ss++bil_val_ss) [bil_load_from_mem_EQ_NONE] >>
+    Cases_on `en = NoEndian` >> (
+       FULL_SIMP_TAC (std_ss++boolSimps.CONJ_ss) [bil_number_of_mem_splits_ID]
+    )
+  ) >>
+  ASM_SIMP_TAC (std_ss++bil_val_ss) [] >>
+  METIS_TAC [type_of_bil_load_from_mem]
+) >- (
+  ASM_SIMP_TAC (std_ss++bil_val_ss) [bil_eval_store_BASIC_REWR] >>
+  rename1 `bil_store_in_mem vt ity mmap en (b2n i)` >>
+  Cases_on `bil_store_in_mem vt ity mmap en (b2n i)` >- (
+    POP_ASSUM MP_TAC >>
+    ASM_SIMP_TAC (std_ss++bil_val_ss) [bil_store_in_mem_EQ_NONE] >>
+    Cases_on `en = NoEndian` >> (
+       FULL_SIMP_TAC (std_ss++boolSimps.CONJ_ss) [bil_number_of_mem_splits_ID]
+    )
+  ) >>
+  ASM_SIMP_TAC (std_ss++bil_val_ss) []
+));
+
 
 
 val _ = export_theory();
